---
title: Double Series Convergence and Summability
tags: [analysis, series, summability]
---

# Double Series

Consider a function $X:\mathbb{N}\times\mathbb{N} \to E$, we abbreviate $X(i,k)$ by $X_{ik}$. The set $\mathbb{N}\times\mathbb{N}$ is countable, that is, there is a bijection $\alpha:\mathbb{N} \to \mathbb{N}\times\mathbb{N}$. If $\alpha$ is such a bijection, $\sum_{n} X_{\alpha(n)}$ is an ordering of the double series $\sum_{i,k} X_{ik}$.

If we fix $j \in \mathbb{N}$ (or $k \in \mathbb{N}$), then $\sum_{k} X_{jk}$ (or $\sum_{j} X_{jk}$) is called the $j^{\text{th}}$ row series (or $j^{\text{th}}$ column series) of $\sum_{j,k} X_{jk}$.

If every row series (or column series) converges, then we consider the series of row sums $\sum_{j} \left( \sum_{k=0}^{\infty} X_{jk} \right)$ (or the series of column sums $\sum_{k} \left( \sum_{j=0}^{\infty} X_{jk} \right)$).

The double series $\sum_{j,k} X_{jk}$ is summable if $\sup_{n \in \mathbb{N}} \sum_{j,k=0}^{n} |X_{jk}| < \infty$.

**Theorem:** Let $\sum_{j,k} X_{jk}$ be a summable double series.

i) Every ordering $\sum_{n} X_{\alpha(n)}$ of $\sum_{j,k} X_{jk}$ converges absolutely to a value $s \in E$ which is independent of $\alpha$.

ii) The series of row sums $\sum_{j} \left( \sum_{k=0}^{\infty} X_{jk} \right)$ and column sums $\sum_{k} \left( \sum_{j=0}^{\infty} X_{jk} \right)$ converges absolutely, and
$$\sum_{j=0}^{\infty} \left( \sum_{k=0}^{\infty} X_{jk} \right) = \sum_{k=0}^{\infty} \left( \sum_{j=0}^{\infty} X_{jk} \right) = S$$

**Proof:** Set $M = \sup_{n \in \mathbb{N}} \sum_{j,k=0}^{n} |X_{jk}| < \infty$. Let $\alpha:\mathbb{N} \to \mathbb{N}\times\mathbb{N}$ be a bijection and $N \in \mathbb{N}$.

Then there is some $K \in \mathbb{N}$ such that
$$\{\alpha(0), \dots, \alpha(N)\} \subseteq \{(0,0), (1,0), \dots, (K,0), \dots, (0,K), \dots, (K,K)\}.$$
This implies
$$\sum_{n=0}^{N} |X_{\alpha(n)}| \le \sum_{j,k=0}^{K} |X_{jk}| \le M$$
and therefore $\sum_{n} X_{\alpha(n)}$ is absolutely convergent.

Now let $\beta: \mathbb{N} \to \mathbb{N}\times\mathbb{N}$ be an other bijection. Then $\sigma := \alpha^{-1} \circ \beta$ is a permutation of $\mathbb{N}$. Set $Y_m := X_{\beta(m)}$ for all $m \in \mathbb{N}$. Then
$$Y_{\sigma(n)} = X_{\beta(\sigma(n))} = X_{\alpha(n)} \quad n \in \mathbb{N}$$
Thus $\sum_{n} X_{\beta(n)}$ is a rearrangement of $\sum_{n} X_{\alpha(n)}$. Since we already know that $\sum_{n} X_{\alpha(n)}$ converges absolutely, the rest of the statement follows from the rearrangement theorem.

## Recommended Reading
- **Writing Proofs in Analysis** by Jonathan M. Kane (Match: 0.68)
- **Real Analysis** by Patrick Fitzpatrick (Match: 0.68)
- **Analysis I** by H. Amann (Match: 0.68)
