---
title: Inequalities Notes
tags: [mathematics, analysis, inequalities]
---

The first inequality example:
$$\log\left(\frac{\xi^p}{p} + \frac{\eta^{p'}}{p'}\right) \geq \frac{1}{p} \log\left(\xi^{p}\right) + \frac{1}{p'} \log\left(\eta^{p'}\right) \quad (\text{since } \log \text{ is convex}).$$
$$= \log\xi + \log\eta = \log(\xi\cdot\eta) \quad (\text{because exp is increasing}) \text{ we have:}$$ 
$$\frac{\xi^p}{p} + \frac{\eta^{p'}}{p'} \geq \xi\cdot\eta \qquad (1) \quad \text{Youngsche Ungleichung}$$

For $n \in \mathbb{N}^*$ and $x_j \in \mathbb{R}^+$, $1 \le j \le n$ it holds:
$$\sqrt[n]{\prod_{j=1}^{n} x_j} \le \frac{1}{n} \sum_{j=1}^{n} x_j \qquad (2) \quad \text{GM} \le \text{AH}$$

For $n=1$ this is true. Let (2) be true for $n \in \mathbb{N}^*$, then we get
$$\prod_{j=1}^{n} x_j \le \left(\frac{1}{n} \sum_{j=1}^{n} x_j\right)^{n}.$$ 
And $\sqrt[n+1]{\prod_{j=1}^{n+1} x_j} \le \frac{1}{n+1} \sum_{j=1}^{n+1} x_j$, so we have $p=1+\frac{1}{n}$, $p'=n+1$.

$$\sqrt[n+1]{\prod_{j=1}^{n} x_j} \cdot \sqrt[n+1]{x_{n+1}} \le \frac{1}{n} \sum_{j=1}^{n} x_j \cdot \frac{1}{n+1} x_{n+1}.$$ 
For $p \in (1,\infty)$ and $x = (x_1,\ldots,x_n) \in \mathbb{K}^n$ let:
$$|x|_p := \left(\sum_{j=1}^{n} |x_j|^p\right)^{1/p}. \quad \text{Then it holds}$$ 
$$\sum_{j=1}^{n} |x_j y_j| \le |x|_p |y|_{p'}, \quad x,y\in\mathbb{K}^n \quad \text{H\"oldersche Ungleichung}$$ 
For the single summands we have with (1):
$$\frac{|x_j|}{|x|_p} \frac{|y_j|}{|y|_{p'}} < \frac{1}{p} \frac{|x_j|^p}{|x|_p^p} + \frac{1}{p'} \frac{|y_j|^{p'}}{|y|_{p'}^{p'}}, \quad 1 \le j \le n,$$ 
The sum of all these inequalities yields:
$$\sum_{j=1}^{n} \frac{|x_j y_j|}{|x|_p |y|_{p'}} \le \sum_{j=1}^{n} \left( \frac{1}{p} \frac{|x_j|^p}{|x|_p^p} + \frac{1}{p'} \frac{|y_j|^{p'}}{|y|_{p'}^{p'}} \right) = \frac{1}{p} + \frac{1}{p'} = 1.$$ 

For $p\in(1,\infty)$ it holds
$$|x+y|_p \le |x|_p + |y|_p$$

The triangle inequality gives us:
$$|x+y|_p^p = \sum_{j=1}^{n} |x_j+y_j|^p = \sum_{j=1}^{n} |x_j+y_j|^{p-1} |x_j+y_j| \le \sum_{j=1}^{n} |x_j+y_j|^{p-1} (|x_j| + |y_j|)$$ 
$$= \sum_{j=1}^{n} |x_j+y_j|^{p-1} |x_j| + \sum_{j=1}^{n} |x_j+y_j|^{p-1} |y_j|.$$

With the H\"older inequality we get
$$|x+y|_p^p \le |x|_p \left(\sum_{j=1}^{n} |x_j+y_j|^p\right)^{p/p'} + |y|_p \left(\sum_{j=1}^{n} |x_j+y_j|^p\right)^{p/p'} = \dots$$

(because $p' = \frac{p}{p-1}$)
$$|x|_p + |y|_p\left(\frac{|x+y|_p^p}{|x+y|_p^{p'}}\right) \quad \text{and divide with } |x+y|_p^{p/p'}.$$

## Recommended Reading
- **Lineare Funktionalanalysis Eine Anwendungsorientierte Einfhrung** by Hans Wilhelm Alt (Match: 0.69)
- **Analysis** by Lieb & Loss (Match: 0.69)
- **Problems in real analysis** by Teodora-Liliana RÄƒdulescu (Match: 0.69)
